refactor to use modules

CAD.dfy
@@ -1,765 +1,787 @@
 // RUN: /compile:0 /rlimit:500000
 
-datatype Expr =
-    | Empty
-    | Unit
-    | Translate(r: real, e: Expr)
-    | Scale(r: real, e: Expr)
-    | Home(r: real, e: Expr)
-    | Intersect(e1: Expr, e2: Expr)
-    | Union(e1: Expr, e2: Expr)
-    | Difference(e1: Expr, e2: Expr)
-
-predicate InOpenInterval(a: real, b: real, x: real)
-{
-    a < x < b
-}
-
-function OpenInterval(a: real, b: real): iset<real>
-{
-    iset x | InOpenInterval(a, b, x)
-}
-
-predicate InClosedInterval(a: real, b: real, x: real)
-{
-    a <= x <= b
-}
-
-function ClosedInterval(a: real, b: real): iset<real>
-{
-    iset x | InClosedInterval(a, b, x)
-}
-
-function DenoteTranslate(r: real, S: iset<real>): iset<real>
-{
-    iset x {:nowarn} | x - r in S
-}
-
-
-function DenoteScale(r: real, S: iset<real>): iset<real>
-{
-    if r == 0.0 then iset{}
-    else iset x {:nowarn} | x / r in S
-}
-
-
-// The following example shows that the semantics of difference cannot
-// be A - B, but must be A - cl(B)
-
-function HalfOpenInterval(): iset<real>
-{
-    OpenInterval(-0.5, 0.5) - OpenInterval(0.0, 0.5)
-}
-
-// Construct the singleton set containing 0.0
-lemma Bad()
-    ensures forall x | x in HalfOpenInterval() && x in DenoteScale(-1.0, HalfOpenInterval()) :: x == 0.0
-{}
-
-
-lemma EmptyBounded()
-    ensures Bounded(iset{})
-{
-    assert IsLB(0.0, iset{});
-    assert IsUB(0.0, iset{});
-}
-
-lemma OpenIntervalBounded(a: real, b: real)
-    ensures Bounded(OpenInterval(a, b))
-{
-    assert IsLB(a, OpenInterval(a, b));
-    assert IsUB(b, OpenInterval(a, b));
-}
-
-lemma DenoteTranslateBounded(r: real, S: iset<real>)
-    requires Bounded(S)
-    ensures Bounded(DenoteTranslate(r, S))
-{
-    var a :| IsLB(a, S);
-    var b :| IsUB(b, S);
-    assert IsLB(a + r, DenoteTranslate(r, S));
-    assert IsUB(b + r, DenoteTranslate(r, S));
-}
-
-lemma DenoteScaleBounded(r: real, S: iset<real>)
-    requires Bounded(S)
-    ensures Bounded(DenoteScale(r, S))
-{
-    var a :| IsLB(a, S);
-    var b :| IsUB(b, S);
-    if r == 0.0 {
-        EmptyBounded();
-    } else if r > 0.0 {
-        assert IsLB(a * r, DenoteScale(r, S));
-        assert IsUB(b * r, DenoteScale(r, S));
-    } else {
-        assert IsLB(b * r, DenoteScale(r, S));
-        assert IsUB(a * r, DenoteScale(r, S));
-    }
-}
-
-lemma IntersectBounded(A: iset<real>, B: iset<real>)
-    requires Bounded(A)
-    ensures Bounded(A * B)
-{
-    var a :| IsLB(a, A);
-    var b :| IsUB(b, A);
-    assert IsLB(a, A * B);
-    assert IsUB(b, A * B);
-}
-
-lemma UnionBounded(A: iset<real>, B: iset<real>)
-    requires Bounded(A) && Bounded(B)
-    ensures Bounded(A + B)
-{
-    var la :| IsLB(la, A);
-    var ua :| IsUB(ua, A);
-
-    var lb :| IsLB(lb, B);
-    var ub :| IsUB(ub, B);
-
-    assert IsLB(min(la, lb), A + B);
-    assert IsUB(max(ua, ub), A + B);
-}
-
-lemma DifferenceBounded(A: iset<real>, B: iset<real>)
-    requires Bounded(A)
-    ensures Bounded(A - B)
-{
-    assert A - B == A * (R() - B);
-    IntersectBounded(A, R() - B);
-}
-
-// ⦇e⦈
-function OpenDenote(e: Expr): (S: iset<real>)
-    ensures Bounded(S)
-{
-    match e
-        case Empty =>
-            EmptyBounded();
-            iset{}
-        case Unit =>
-            OpenIntervalBounded(0.0, 1.0);
-            OpenInterval(0.0, 1.0)
-        case Translate(r,e) =>
-            DenoteTranslateBounded(r, OpenDenote(e));
-            DenoteTranslate(r, OpenDenote(e))
-        case Home(r, e) => var S' := OpenDenote(e);
-            if S' == iset{} then
-                EmptyBounded();
-                iset{}
-            else
-                DenoteTranslateBounded(RelPos(r, S'), S');
-                DenoteTranslate(RelPos(r, S'), S')
-        case Scale(r,e) =>
-            DenoteScaleBounded(r, OpenDenote(e));
-            DenoteScale(r, OpenDenote(e))
-        case Intersect(e1,e2) =>
-            IntersectBounded(OpenDenote(e1), OpenDenote(e2));
-            OpenDenote(e1) * OpenDenote(e2)
-        case Union(e1,e2) =>
-            UnionBounded(OpenDenote(e1), OpenDenote(e2));
-            OpenDenote(e1) + OpenDenote(e2)
-        case Difference(e1,e2) =>
-            DifferenceBounded(OpenDenote(e1), Closure(OpenDenote(e2)));
-            OpenDenote(e1) - Closure(OpenDenote(e2))
-}
-
-
-function abs(r: real): real
-{
-    if r < 0.0 then
-        - r
-    else r
-}
-
-function min(a: real, b: real): real
-{
-    if a < b then
-        a
-    else
-        b
-}
-
-function max(a: real, b: real): real
-{
-    if a > b then
-        a
-    else
-        b
-}
-
-predicate InBall(center: real, r: real, x: real)
-{
-    abs(center - x) < r
-}
-
-function Ball(center: real, r: real): iset<real>
-{
-    iset x | InBall(center, r, x)
-}
-
-predicate InClosure(x: real, S: iset<real>)
-{
-    forall eps | eps > 0.0 :: !(Ball(x, eps) !! S)
-}
-
-function Closure(S: iset<real>): iset<real>
-{
-    iset x | InClosure(x, S)
-}
-
-// ⟦e⟧
-function Denote(e: Expr): iset<real>
-{
-    Closure(OpenDenote(e))
-}
-
-lemma ISetNonEmpty<A>(x: A, S: iset<A>)
-    requires x in S
-    ensures S != iset{}
-{}
-
-lemma ClosureOpenInterval(a: real, b: real)
-    requires a < b
-    ensures Closure(OpenInterval(a, b)) == ClosedInterval(a, b)
-{
-    forall x | x in Closure(OpenInterval(a, b))
-        ensures x in ClosedInterval(a, b)
+module PreludeModule {
+    function abs(r: real): real
     {
-        if x < a {
-            var eps := (a - x) / 2.0;
-            var y :| y in Ball(x, eps) * OpenInterval(a, b);
-        } else if x > b {
-            var eps := (x - b) / 2.0;
-            var y :| y in Ball(x, eps) * OpenInterval(a, b);
-        }
+        if r < 0.0 then
+            - r
+        else r
+    }
+    
+    function min(a: real, b: real): real
+    {
+        if a < b then
+            a
+        else
+            b
+    }
+    
+    function max(a: real, b: real): real
+    {
+        if a > b then
+            a
+        else
+            b
     }
 
-    forall x | x in ClosedInterval(a, b)
-        ensures x in Closure(OpenInterval(a, b))
+    lemma ISetNonEmpty<A>(x: A, S: iset<A>)
+        requires x in S
+        ensures S != iset{}
+    {}
+}
+
+module RealModule {
+    import opened PreludeModule
+
+    predicate InOpenInterval(a: real, b: real, x: real)
     {
-        forall eps | eps > 0.0
-            ensures Ball(x, eps) * OpenInterval(a, b) != iset{}
+        a < x < b
+    }
+    
+    function OpenInterval(a: real, b: real): iset<real>
+    {
+        iset x | InOpenInterval(a, b, x)
+    }
+    
+    predicate InClosedInterval(a: real, b: real, x: real)
+    {
+        a <= x <= b
+    }
+    
+    function ClosedInterval(a: real, b: real): iset<real>
+    {
+        iset x | InClosedInterval(a, b, x)
+    }
+
+    predicate InTranslatedSet(r: real, S: iset<real>, x: real)
+    {
+        x - r in S
+    }
+
+    function TranslateSet(r: real, S: iset<real>): iset<real>
+    {
+        iset x | InTranslatedSet(r, S, x)
+    }
+    
+    predicate InScaledSet(r: real, S: iset<real>, x: real)
+        requires r != 0.0
+    {
+        x / r in S
+    }
+
+    function ScaleSet(r: real, S: iset<real>): iset<real>
+    {
+        if r == 0.0 then iset{}
+        else iset x | InScaledSet(r, S, x)
+    }
+
+    predicate IsUB(x: real, S: iset<real>)
+    {
+        forall y | y in S :: y <= x
+    }
+    
+    predicate IsLUB(x: real, S: iset<real>)
+    {
+        IsUB(x, S) && forall x' | IsUB(x', S) :: x <= x'
+    }
+    
+    lemma {:axiom} LUBExists(S: iset<real>)
+        requires exists x :: x in S
+        requires exists x :: IsUB(x, S)
+        ensures exists x :: IsLUB(x, S)
+    
+    function LUB(S: iset<real>): real
+        requires exists x :: x in S
+        requires exists x :: IsUB(x, S)
+    {
+        LUBExists(S);
+        var x :| IsLUB(x, S);
+        x
+    }
+    
+    predicate IsLB(x: real, S: iset<real>)
+    {
+        forall y | y in S :: x <= y
+    }
+    
+    predicate IsGLB(x: real, S: iset<real>)
+    {
+        IsLB(x, S) && forall x' | IsLB(x', S) :: x' <= x
+    }
+    
+    lemma GLBExists(S: iset<real>)
+        requires exists x :: IsLB(x, S)
+        requires exists x :: x in S
+        ensures exists x :: IsGLB(x, S)
+    {
+        var x :| x in S;
+        var y :| IsLB(y, S);
+        var LBs := iset x | IsLB(x, S);
+        assert IsUB(x, LBs);
+        assert y in LBs;
+        LUBExists(LBs);
+        var x' :| IsLUB(x', LBs);
+        assert IsUB(x', LBs);
+    
+        forall y | IsLB(y, S)
+            ensures y <= x'
         {
-            if x == a {
-                var d := min(eps, b - a) / 2.0;
-                assert x + d in Ball(a, eps);
-                ISetNonEmpty(x + d, Ball(a, eps) * OpenInterval(a, b));
-            } else if x == b {
-                var d := min(eps, b - a) / 2.0;
-                ISetNonEmpty(x - d, Ball(b, eps) * OpenInterval(a, b));
-            } else {
-                ISetNonEmpty(x, Ball(x, eps) * OpenInterval(a, b));
+            assert y in LBs;
+        }
+        forall y | y in S
+            ensures x' <= y
+        {
+            if y < x' {
+                assert IsUB(y, LBs);
+                assert false;
             }
         }
+        assert IsGLB(x', S);
     }
-}
-
-lemma ClosureUnion(A: iset<real>, B: iset<real>)
-    ensures Closure(A + B) == Closure(A) + Closure(B)
-{ }
-
-
-
-
-lemma CloseAdjacentOpenIntervals(a: real, b: real, c: real)
-    requires a <= b <= c
-    ensures Closure(OpenInterval(a, b) + OpenInterval(b, c)) == Closure(OpenInterval(a, c))
-{
-    if a == b || b == c { return; }
-
-    ClosureUnion(OpenInterval(a,b), OpenInterval(b,c));
-    ClosureOpenInterval(a, c);
-    ClosureOpenInterval(a, b);
-    ClosureOpenInterval(b, c);
-}
-
-lemma UnionUnitTest()
-    ensures Denote(Union(Unit, Translate(1.0, Unit))) == Denote(Scale(2.0, Unit))
-{
-    calc {
-        Denote(Union(Unit, Translate(1.0, Unit)));
-        == Closure(OpenDenote(Union(Unit, Translate(1.0, Unit))));
-        == Closure(OpenInterval(0.0, 1.0) + DenoteTranslate(1.0, OpenInterval(0.0, 1.0)));
-        == Closure(OpenInterval(0.0, 1.0) + OpenInterval(1.0, 2.0));
-        == { CloseAdjacentOpenIntervals(0.0, 1.0, 2.0); }
-           Closure(OpenInterval(0.0, 2.0));
-        == Closure(DenoteScale(2.0, OpenInterval(0.0, 1.0)));
-        == Closure(OpenDenote(Scale(2.0, Unit)));
-        == Denote(Scale(2.0, Unit));
-    }
-}
-
-lemma DiffUnitTest()
-    ensures Denote(Difference(Unit, Translate(1.0, Unit))) == Denote(Unit)
-{
-    calc {
-        Denote(Difference(Unit, Translate(1.0, Unit)));
-        Closure(OpenInterval(0.0, 1.0) - Closure(DenoteTranslate(1.0, OpenInterval(0.0, 1.0))));
-        == Closure(OpenInterval(0.0, 1.0) - Closure(OpenInterval(1.0, 2.0)));
-        == { ClosureOpenInterval(1.0, 2.0); }
-           Closure(OpenInterval(0.0, 1.0) - ClosedInterval(1.0, 2.0));
-        == Denote(Unit);
-    }
-}
-
-// Look ma, no proof!
-lemma IntersectUnitTest()
-    ensures Denote(Intersect(Unit, Translate(1.0, Unit))) == Denote(Empty)
-{}
-
-predicate InInterior(x: real, S: iset<real>)
-{
-    exists eps | eps > 0.0 :: Ball(x, eps) <= S
-}
-
-function Interior(S: iset<real>): iset<real>
-{
-    iset x | InInterior(x, S)
-}
-
-predicate Open(S: iset<real>)
-{
-    forall x | x in S :: InInterior(x, S)
-}
-
-lemma OpenIntervalOpen(a: real, b: real)
-    requires a < b
-    ensures Open(OpenInterval(a, b))
-{
-    var S := OpenInterval(a, b);
-    forall x | x in S
-        ensures exists eps | eps > 0.0 :: Ball(x, eps) <= S
+    
+    
+    function GLB(S: iset<real>): real
+        requires exists x :: x in S
+        requires exists x :: IsLB(x, S)
     {
-        var eps := min((x - a) / 2.0, (b - x) / 2.0);
-        assert Ball(x, eps) <= S;
+        GLBExists(S);
+        var x :| IsGLB(x, S);
+        x
     }
-}
-
-lemma DenoteTranslateOpen(r: real, S: iset<real>)
-    requires Open(S)
-    ensures Open(DenoteTranslate(r, S))
-{
-    var S' := DenoteTranslate(r, S);
-    forall x | x in S'
-        ensures exists eps | eps > 0.0 :: Ball(x, eps) <= S'
+    
+    predicate NonEmpty(S: iset<real>)
     {
-        var y := x - r;
-        assert y in S;
-        var eps :| eps > 0.0 && Ball(y, eps) <= S;
-
-        assert Ball(x, eps) <= S';
+        exists x :: x in S
     }
-}
-
-lemma DenoteScaleOpen(r: real, S: iset<real>)
-    requires Open(S)
-    ensures Open(DenoteScale(r, S))
-{
-    if r == 0.0 { return; }
-    var S' := DenoteScale(r, S);
-    forall x | x in S'
-        ensures exists eps | eps > 0.0 :: Ball(x, eps) <= S'
+    
+    predicate InBall(center: real, r: real, x: real)
     {
-        var y := x / r;
-        assert y in S;
-        var eps :| eps > 0.0 && Ball(y, eps) <= S;
-
-        assert Ball(x, abs(r) * eps) <= S';
+        abs(center - x) < r
     }
-}
-
-function R(): iset<real>
-{
-    iset x {:nowarn} | true
-}
-
-predicate Closed(S: iset<real>)
-{
-    S == Closure(S)
-}
-
-lemma ClosureSubset(S: iset<real>)
-    ensures S <= Closure(S)
-{}
-
-lemma ClosureIdempotent(S: iset<real>)
-    ensures Closure(Closure(S)) == Closure(S)
-{
-    forall x | x in Closure(Closure(S))
-        ensures x in Closure(S)
+    
+    function Ball(center: real, r: real): iset<real>
     {
-        forall eps | eps > 0.0
-            ensures !(Ball(x, eps) !! S)
+        iset x | InBall(center, r, x)
+    }
+    
+    predicate InClosure(x: real, S: iset<real>)
+    {
+        forall eps | eps > 0.0 :: !(Ball(x, eps) !! S)
+    }
+    
+    function Closure(S: iset<real>): iset<real>
+    {
+        iset x | InClosure(x, S)
+    }
+
+    lemma ClosureOpenInterval(a: real, b: real)
+        requires a < b
+        ensures Closure(OpenInterval(a, b)) == ClosedInterval(a, b)
+    {
+        forall x | x in Closure(OpenInterval(a, b))
+            ensures x in ClosedInterval(a, b)
         {
-            var y :| y in Ball(x, eps / 2.0) && y in Closure(S);
-            var z :| z in Ball(y, eps / 2.0) && z in S;
-        }
-    }
-}
-
-lemma ClosureClosed(S: iset<real>)
-    ensures Closed(Closure(S))
-{
-    ClosureIdempotent(S);
-}
-
-
-lemma DisjointIntersectionEmpty<T>(A: iset<T>, B: iset<T>)
-    requires A * B == iset{}
-    ensures A !! B
-{
-    forall a, b | a in A && b in B
-        ensures a != b
-    {
-        if a == b {
-            assert a in A * B;
-            ISetNonEmpty(a, A * B);
-        }
-    }
-}
-
-lemma ComplementClosedOpen(S: iset<real>)
-    requires Closed(S)
-    ensures Open(R() - S)
-{
-    var D := R() - S;
-    forall x | x in D
-        ensures exists eps | eps > 0.0 :: Ball(x, eps) <= D
-    {
-        assert x !in Closure(S);
-        var eps :| eps > 0.0 && Ball(x, eps) * S == iset{};
-        DisjointIntersectionEmpty(Ball(x, eps), S);
-        assert Ball(x, eps) <= D;
-    }
-}
-
-lemma IntersectOpen(S1: iset<real>, S2: iset<real>)
-    requires Open(S1) && Open(S2)
-    ensures Open(S1 * S2)
-{}
-
-lemma DifferenceOpen(S1: iset<real>, S2: iset<real>)
-    requires Open(S1)
-    ensures Open(S1 - Closure(S2))
-{
-    assert S1 - Closure(S2) == S1 * (R() - Closure(S2));
-    ClosureClosed(S2);
-    ComplementClosedOpen(Closure(S2));
-    IntersectOpen(S1, R() - Closure(S2));
-}
-
-
-lemma OpenDenoteOpen(e: Expr)
-    ensures Open(OpenDenote(e))
-{
-    match e {
-        case Empty =>
-        case Unit => OpenIntervalOpen(0.0, 1.0);
-        case Translate(r, e) => DenoteTranslateOpen(r, OpenDenote(e));
-        case Home(r, e) => var S := OpenDenote(e);
-            if S != iset{} {
-                DenoteTranslateOpen(RelPos(r, S), S);
+            if x < a {
+                var eps := (a - x) / 2.0;
+                var y :| y in Ball(x, eps) * OpenInterval(a, b);
+            } else if x > b {
+                var eps := (x - b) / 2.0;
+                var y :| y in Ball(x, eps) * OpenInterval(a, b);
             }
-        case Scale(r, e) => { DenoteScaleOpen(r, OpenDenote(e)); }
-        case Intersect(e1, e2) => {}
-        case Union(e1, e2) => {}
-        case Difference(e1, e2) => { DifferenceOpen(OpenDenote(e1), OpenDenote(e2)); }
-    }
-}
-
-predicate NoIsolatedPoints(S: iset<real>)
-{
-    forall x, eps | x in S && eps > 0.0 :: !((Ball(x, eps) - iset{x}) !! S)
-}
-
-lemma DenoteNoIsolatedPoints(e: Expr)
-    ensures NoIsolatedPoints(Denote(e))
-{
-    forall x, eps | x in Denote(e) && eps > 0.0
-        ensures exists z :: z in Ball(x, eps) && z != x && z in Denote(e)
-    {
-        assert !(OpenDenote(e) !! Ball(x, eps / 2.0));
-        var y :| y in OpenDenote(e) && y in Ball(x, eps / 2.0);
-        if x == y {
-            OpenDenoteOpen(e);
-            var eps' :| eps' > 0.0 && Ball(y, eps') <= OpenDenote(e);
-            var eps'' := min(eps, eps') / 2.0;
-            var z := x + eps'';
-            assert z in Ball(y, eps');
-            assert z in Denote(e);
-        } else {
-            assert y in Denote(e);
         }
-
-    }
-}
-
-predicate HasNearbyPointInInterior(S: iset<real>, x: real, eps: real)
-{
-    exists x', eps' | eps' > 0.0 :: Ball(x', eps') <= (Ball(x, eps) * S)
-}
-
-predicate NoInfinitelyThinFeatures(S: iset<real>)
-{
-    forall x, eps | x in S && eps > 0.0 ::
-        HasNearbyPointInInterior(S, x, eps)
-}
-
-lemma DenoteNoInfinitelyThinFeatures(e: Expr)
-    ensures NoInfinitelyThinFeatures(Denote(e))
-{
-    var S := Denote(e);
-    forall x, eps | x in S && eps > 0.0
-        ensures HasNearbyPointInInterior(S, x, eps)
-    {
-        assert x in Closure(OpenDenote(e));
-        var x' :| x' in Ball(x, eps) && x' in OpenDenote(e);
-        OpenDenoteOpen(e);
-        var eps' :| eps' > 0.0 && Ball(x', eps') <= OpenDenote(e);
-
-        var eps'' := min(eps', eps - abs(x - x'));
-        assert Ball(x', eps'') <= OpenDenote(e);
-    }
-}
-
-predicate AlternativeNoInfinitelyThinFeatures(S: iset<real>)
-{
-    S <= Closure(Interior(S))
-}
-
-lemma AlternativeNoInfinitelyThinFeaturesEquiv(S: iset<real>)
-    ensures AlternativeNoInfinitelyThinFeatures(S) <==> NoInfinitelyThinFeatures(S)
-{
-    if AlternativeNoInfinitelyThinFeatures(S) {
-        forall x, eps | x in S && eps > 0.0
-            ensures HasNearbyPointInInterior(S, x, eps)
-        {
-            var x' :| x' in Ball(x, eps) && x' in Interior(S);
-            var eps' :| eps' > 0.0 && Ball(x', eps') <= S;
-            var eps'' := min(eps', eps - abs(x - x'));
-            assert Ball(x', eps'') <= Ball(x, eps);
-        }
-    }
-
-    if NoInfinitelyThinFeatures(S) {
-        forall x | x in S
-            ensures x in Closure(Interior(S))
+    
+        forall x | x in ClosedInterval(a, b)
+            ensures x in Closure(OpenInterval(a, b))
         {
             forall eps | eps > 0.0
-                ensures !(Ball(x, eps) !! Interior(S))
+                ensures Ball(x, eps) * OpenInterval(a, b) != iset{}
             {
-                assert HasNearbyPointInInterior(S, x, eps);
-                var x', eps' :| eps' > 0.0 && Ball(x', eps') <= (Ball(x, eps) * S);
-                assert x' in Ball(x', eps');
+                if x == a {
+                    var d := min(eps, b - a) / 2.0;
+                    assert x + d in Ball(a, eps);
+                    ISetNonEmpty(x + d, Ball(a, eps) * OpenInterval(a, b));
+                } else if x == b {
+                    var d := min(eps, b - a) / 2.0;
+                    ISetNonEmpty(x - d, Ball(b, eps) * OpenInterval(a, b));
+                } else {
+                    ISetNonEmpty(x, Ball(x, eps) * OpenInterval(a, b));
+                }
             }
         }
     }
-}
-
-predicate IsUB(x: real, S: iset<real>)
-{
-    forall y | y in S :: y <= x
-}
-
-predicate IsLUB(x: real, S: iset<real>)
-{
-    IsUB(x, S) && forall x' | IsUB(x', S) :: x <= x'
-}
-
-lemma {:axiom} LUBExists(S: iset<real>)
-    requires exists x :: x in S
-    requires exists x :: IsUB(x, S)
-    ensures exists x :: IsLUB(x, S)
-
-function LUB(S: iset<real>): real
-    requires exists x :: x in S
-    requires exists x :: IsUB(x, S)
-{
-    LUBExists(S);
-    var x :| IsLUB(x, S);
-    x
-}
-
-predicate IsLB(x: real, S: iset<real>)
-{
-    forall y | y in S :: x <= y
-}
-
-predicate IsGLB(x: real, S: iset<real>)
-{
-    IsLB(x, S) && forall x' | IsLB(x', S) :: x' <= x
-}
-
-lemma GLBExists(S: iset<real>)
-    requires exists x :: IsLB(x, S)
-    requires exists x :: x in S
-    ensures exists x :: IsGLB(x, S)
-{
-    var x :| x in S;
-    var y :| IsLB(y, S);
-    var LBs := iset x | IsLB(x, S);
-    assert IsUB(x, LBs);
-    assert y in LBs;
-    LUBExists(LBs);
-    var x' :| IsLUB(x', LBs);
-    assert IsUB(x', LBs);
-
-    forall y | IsLB(y, S)
-        ensures y <= x'
+    
+    lemma ClosureUnion(A: iset<real>, B: iset<real>)
+        ensures Closure(A + B) == Closure(A) + Closure(B)
+    { }
+    
+    lemma ClosureEmpty()
+        ensures Closure(iset{}) == iset{}
     {
-        assert y in LBs;
-    }
-    forall y | y in S
-        ensures x' <= y
-    {
-        if y < x' {
-            assert IsUB(y, LBs);
+        forall x | x in Closure(iset{})
+            ensures x in iset{}
+        {
+            var x' :| x' in Ball(x, 1.0) && x' in iset{};
             assert false;
         }
     }
-    assert IsGLB(x', S);
-}
 
-
-function GLB(S: iset<real>): real
-    requires exists x :: x in S
-    requires exists x :: IsLB(x, S)
-{
-    GLBExists(S);
-    var x :| IsGLB(x, S);
-    x
-}
-
-predicate Bounded(S: iset<real>)
-{
-    && (exists x :: IsLB(x, S))
-    && (exists x :: IsUB(x, S))
-}
-
-predicate NonEmpty(S: iset<real>)
-{
-    exists x :: x in S
-}
-
-function BBox(S: iset<real>): (real, real)
-    requires NonEmpty(S) && Bounded(S)
-{
-    GLBExists(S);
-    LUBExists(S);
-    var a :| IsGLB(a, S);
-    var b :| IsLUB(b, S);
-    (a, b)
-}
-
-function RelPos(r: real, S: iset<real>): real
-    requires NonEmpty(S) && Bounded(S)
-{
-    var (a, b) := BBox(S);
-    a + r * (b - a)
-}
-
-
-
-predicate Equiv(e1: Expr, e2: Expr)
-{
-    Denote(e1) == Denote(e2)
-}
-
-lemma SelfUnion(e: Expr)
-    ensures Equiv(Union(e, e), e)
-{}
-
-lemma SelfIntersect(e: Expr)
-    ensures Equiv(Intersect(e, e), e)
-{}
-
-lemma SelfDifference(e: Expr)
-    ensures Equiv(Difference(e, e), Empty)
-{}
-
-lemma UnionEmpty(e: Expr)
-    ensures Equiv(Union(e, Empty), e)
-{}
-
-lemma IntersectEmpty(e: Expr)
-    ensures Equiv(Intersect(e, Empty), Empty)
-{}
-
-
-lemma ClosureEmpty()
-    ensures Closure(iset{}) == iset{}
-{
-    forall x | x in Closure(iset{})
-        ensures x in iset{}
+    lemma CloseAdjacentOpenIntervals(a: real, b: real, c: real)
+        requires a <= b <= c
+        ensures Closure(OpenInterval(a, b) + OpenInterval(b, c)) == Closure(OpenInterval(a, c))
     {
-        var x' :| x' in Ball(x, 1.0) && x' in iset{};
-        assert false;
+        if a == b || b == c { return; }
+    
+        ClosureUnion(OpenInterval(a,b), OpenInterval(b,c));
+        ClosureOpenInterval(a, c);
+        ClosureOpenInterval(a, b);
+        ClosureOpenInterval(b, c);
+    }
+
+    predicate InInterior(x: real, S: iset<real>)
+    {
+        exists eps | eps > 0.0 :: Ball(x, eps) <= S
+    }
+    
+    function Interior(S: iset<real>): iset<real>
+    {
+        iset x | InInterior(x, S)
+    }
+    
+    predicate Open(S: iset<real>)
+    {
+        forall x | x in S :: InInterior(x, S)
+    }
+    
+    lemma OpenIntervalOpen(a: real, b: real)
+        requires a < b
+        ensures Open(OpenInterval(a, b))
+    {
+        var S := OpenInterval(a, b);
+        forall x | x in S
+            ensures exists eps | eps > 0.0 :: Ball(x, eps) <= S
+        {
+            var eps := min((x - a) / 2.0, (b - x) / 2.0);
+            assert Ball(x, eps) <= S;
+        }
+    }
+    
+    lemma TranslateSetOpen(r: real, S: iset<real>)
+        requires Open(S)
+        ensures Open(TranslateSet(r, S))
+    {
+        var S' := TranslateSet(r, S);
+        forall x | x in S'
+            ensures exists eps | eps > 0.0 :: Ball(x, eps) <= S'
+        {
+            var y := x - r;
+            assert y in S;
+            var eps :| eps > 0.0 && Ball(y, eps) <= S;
+    
+            assert Ball(x, eps) <= S';
+        }
+    }
+    
+    lemma ScaleSetOpen(r: real, S: iset<real>)
+        requires Open(S)
+        ensures Open(ScaleSet(r, S))
+    {
+        if r == 0.0 { return; }
+        var S' := ScaleSet(r, S);
+        forall x | x in S'
+            ensures exists eps | eps > 0.0 :: Ball(x, eps) <= S'
+        {
+            var y := x / r;
+            assert y in S;
+            var eps :| eps > 0.0 && Ball(y, eps) <= S;
+    
+            assert Ball(x, abs(r) * eps) <= S';
+        }
+    }
+
+    function R(): iset<real>
+    {
+        iset x {:nowarn} | true
+    }
+    
+    predicate Closed(S: iset<real>)
+    {
+        S == Closure(S)
+    }
+    
+    lemma ClosureSubset(S: iset<real>)
+        ensures S <= Closure(S)
+    {}
+    
+    lemma ClosureIdempotent(S: iset<real>)
+        ensures Closure(Closure(S)) == Closure(S)
+    {
+        forall x | x in Closure(Closure(S))
+            ensures x in Closure(S)
+        {
+            forall eps | eps > 0.0
+                ensures !(Ball(x, eps) !! S)
+            {
+                var y :| y in Ball(x, eps / 2.0) && y in Closure(S);
+                var z :| z in Ball(y, eps / 2.0) && z in S;
+            }
+        }
+    }
+    
+    lemma ClosureClosed(S: iset<real>)
+        ensures Closed(Closure(S))
+    {
+        ClosureIdempotent(S);
+    }
+    
+    
+    lemma DisjointIntersectionEmpty<T>(A: iset<T>, B: iset<T>)
+        requires A * B == iset{}
+        ensures A !! B
+    {
+        forall a, b | a in A && b in B
+            ensures a != b
+        {
+            if a == b {
+                assert a in A * B;
+                ISetNonEmpty(a, A * B);
+            }
+        }
+    }
+    
+    lemma ComplementClosedOpen(S: iset<real>)
+        requires Closed(S)
+        ensures Open(R() - S)
+    {
+        var D := R() - S;
+        forall x | x in D
+            ensures exists eps | eps > 0.0 :: Ball(x, eps) <= D
+        {
+            assert x !in Closure(S);
+            var eps :| eps > 0.0 && Ball(x, eps) * S == iset{};
+            DisjointIntersectionEmpty(Ball(x, eps), S);
+            assert Ball(x, eps) <= D;
+        }
+    }
+    
+    lemma IntersectOpen(S1: iset<real>, S2: iset<real>)
+        requires Open(S1) && Open(S2)
+        ensures Open(S1 * S2)
+    {}
+    
+    lemma DifferenceOpen(S1: iset<real>, S2: iset<real>)
+        requires Open(S1)
+        ensures Open(S1 - Closure(S2))
+    {
+        assert S1 - Closure(S2) == S1 * (R() - Closure(S2));
+        ClosureClosed(S2);
+        ComplementClosedOpen(Closure(S2));
+        IntersectOpen(S1, R() - Closure(S2));
     }
 }
 
-lemma DifferenceEmpty1(e: Expr)
-    ensures Equiv(Difference(e, Empty), e)
-{
-    ClosureEmpty();
+module BoundedModule {
+    import opened PreludeModule
+    import opened RealModule
+
+    predicate Bounded(S: iset<real>)
+    {
+        && (exists x :: IsLB(x, S))
+        && (exists x :: IsUB(x, S))
+    }
+
+    lemma EmptyBounded()
+        ensures Bounded(iset{})
+    {
+        assert IsLB(0.0, iset{});
+        assert IsUB(0.0, iset{});
+    }
+    
+    lemma OpenIntervalBounded(a: real, b: real)
+        ensures Bounded(OpenInterval(a, b))
+    {
+        assert IsLB(a, OpenInterval(a, b));
+        assert IsUB(b, OpenInterval(a, b));
+    }
+    
+    lemma TranslateSetBounded(r: real, S: iset<real>)
+        requires Bounded(S)
+        ensures Bounded(TranslateSet(r, S))
+    {
+        var a :| IsLB(a, S);
+        var b :| IsUB(b, S);
+        assert IsLB(a + r, TranslateSet(r, S));
+        assert IsUB(b + r, TranslateSet(r, S));
+    }
+    
+    lemma ScaleSetBounded(r: real, S: iset<real>)
+        requires Bounded(S)
+        ensures Bounded(ScaleSet(r, S))
+    {
+        var a :| IsLB(a, S);
+        var b :| IsUB(b, S);
+        if r == 0.0 {
+            EmptyBounded();
+        } else if r > 0.0 {
+            assert IsLB(a * r, ScaleSet(r, S));
+            assert IsUB(b * r, ScaleSet(r, S));
+        } else {
+            assert IsLB(b * r, ScaleSet(r, S));
+            assert IsUB(a * r, ScaleSet(r, S));
+        }
+    }
+    
+    lemma IntersectBounded(A: iset<real>, B: iset<real>)
+        requires Bounded(A)
+        ensures Bounded(A * B)
+    {
+        var a :| IsLB(a, A);
+        var b :| IsUB(b, A);
+        assert IsLB(a, A * B);
+        assert IsUB(b, A * B);
+    }
+    
+    lemma UnionBounded(A: iset<real>, B: iset<real>)
+        requires Bounded(A) && Bounded(B)
+        ensures Bounded(A + B)
+    {
+        var la :| IsLB(la, A);
+        var ua :| IsUB(ua, A);
+    
+        var lb :| IsLB(lb, B);
+        var ub :| IsUB(ub, B);
+    
+        assert IsLB(min(la, lb), A + B);
+        assert IsUB(max(ua, ub), A + B);
+    }
+    
+    lemma DifferenceBounded(A: iset<real>, B: iset<real>)
+        requires Bounded(A)
+        ensures Bounded(A - B)
+    {
+        assert A - B == A * (R() - B);
+        IntersectBounded(A, R() - B);
+    }
+
+    function BBox(S: iset<real>): (real, real)
+        requires NonEmpty(S) && Bounded(S)
+    {
+        GLBExists(S);
+        LUBExists(S);
+        var a :| IsGLB(a, S);
+        var b :| IsLUB(b, S);
+        (a, b)
+    }
 }
 
-lemma DifferenceEmpty2(e: Expr)
-    ensures Equiv(Difference(Empty, e), Empty)
-{}
+module CADModule {
+    import opened PreludeModule
+    import opened RealModule
+    import opened BoundedModule
 
-lemma UnionComm(e1: Expr, e2: Expr)
-    ensures Equiv(Union(e1, e2), Union(e2, e1))
-{}
+    datatype Expr =
+        | Empty
+        | Unit
+        | Translate(r: real, e: Expr)
+        | Scale(r: real, e: Expr)
+        | Home(r: real, e: Expr)
+        | Intersect(e1: Expr, e2: Expr)
+        | Union(e1: Expr, e2: Expr)
+        | Difference(e1: Expr, e2: Expr)
+    
+    
+    // The following example shows that the semantics of difference cannot
+    // be A - B, but must be A - cl(B)
+    
+    function HalfOpenInterval(): iset<real>
+    {
+        OpenInterval(-0.5, 0.5) - OpenInterval(0.0, 0.5)
+    }
+    
+    // Construct the singleton set containing 0.0
+    lemma Bad()
+        ensures forall x | x in HalfOpenInterval() && x in ScaleSet(-1.0, HalfOpenInterval()) :: x == 0.0
+    {}
 
-lemma IntersectComm(e1: Expr, e2: Expr)
-    ensures Equiv(Intersect(e1, e2), Intersect(e2, e1))
-{}
+    // ⦇e⦈
+    function OpenDenote(e: Expr): (S: iset<real>)
+        ensures Bounded(S)
+    {
+        match e
+            case Empty =>
+                EmptyBounded();
+                iset{}
+            case Unit =>
+                OpenIntervalBounded(0.0, 1.0);
+                OpenInterval(0.0, 1.0)
+            case Translate(r,e) =>
+                TranslateSetBounded(r, OpenDenote(e));
+                TranslateSet(r, OpenDenote(e))
+            case Home(r, e) => var S' := OpenDenote(e);
+                TranslateSetBounded(-RelPos(r, S'), S');
+                TranslateSet(-RelPos(r, S'), S')
+            case Scale(r,e) =>
+                ScaleSetBounded(r, OpenDenote(e));
+                ScaleSet(r, OpenDenote(e))
+            case Intersect(e1,e2) =>
+                IntersectBounded(OpenDenote(e1), OpenDenote(e2));
+                OpenDenote(e1) * OpenDenote(e2)
+            case Union(e1,e2) =>
+                UnionBounded(OpenDenote(e1), OpenDenote(e2));
+                OpenDenote(e1) + OpenDenote(e2)
+            case Difference(e1,e2) =>
+                DifferenceBounded(OpenDenote(e1), Closure(OpenDenote(e2)));
+                OpenDenote(e1) - Closure(OpenDenote(e2))
+    }
 
-lemma UnionAssoc(e1: Expr, e2: Expr, e3: Expr)
-    ensures Equiv(Union(e1, Union(e2, e3)), Union(Union(e1, e2), e3))
-{
-    assert
-        OpenDenote(e1) + (OpenDenote(e2) + OpenDenote(e3)) ==
-        (OpenDenote(e1) + OpenDenote(e2)) + OpenDenote(e3);
-}
+    // ⟦e⟧
+    function Denote(e: Expr): iset<real>
+    {
+        Closure(OpenDenote(e))
+    }
 
-lemma IntersectAssoc(e1: Expr, e2: Expr, e3: Expr)
-    ensures Equiv(Intersect(e1, Intersect(e2, e3)), Intersect(Intersect(e1, e2), e3))
-{
-    assert
-        OpenDenote(e1) * (OpenDenote(e2) * OpenDenote(e3)) ==
-        (OpenDenote(e1) * OpenDenote(e2)) * OpenDenote(e3);
-}
-
-lemma IntersectDifference(e1: Expr, e2: Expr)
-    ensures Equiv(Intersect(e1, e2), Difference(e1, Difference(e1, e2)));
-{
-    calc {
-        Denote(Intersect(e1, e2));
-        Closure(OpenDenote(Intersect(e1, e2)));
-        Closure(OpenDenote(e1) * OpenDenote(e2));
+    lemma UnionUnitTest()
+        ensures Denote(Union(Unit, Translate(1.0, Unit))) == Denote(Scale(2.0, Unit))
+    {
+        calc {
+            Denote(Union(Unit, Translate(1.0, Unit)));
+            == Closure(OpenDenote(Union(Unit, Translate(1.0, Unit))));
+            == Closure(OpenInterval(0.0, 1.0) + TranslateSet(1.0, OpenInterval(0.0, 1.0)));
+            == Closure(OpenInterval(0.0, 1.0) + OpenInterval(1.0, 2.0));
+            == { CloseAdjacentOpenIntervals(0.0, 1.0, 2.0); }
+               Closure(OpenInterval(0.0, 2.0));
+            == Closure(ScaleSet(2.0, OpenInterval(0.0, 1.0)));
+            == Closure(OpenDenote(Scale(2.0, Unit)));
+            == Denote(Scale(2.0, Unit));
+        }
+    }
+    
+    lemma DiffUnitTest()
+        ensures Denote(Difference(Unit, Translate(1.0, Unit))) == Denote(Unit)
+    {
+        calc {
+            Denote(Difference(Unit, Translate(1.0, Unit)));
+            Closure(OpenInterval(0.0, 1.0) - Closure(TranslateSet(1.0, OpenInterval(0.0, 1.0))));
+            == Closure(OpenInterval(0.0, 1.0) - Closure(OpenInterval(1.0, 2.0)));
+            == { ClosureOpenInterval(1.0, 2.0); }
+               Closure(OpenInterval(0.0, 1.0) - ClosedInterval(1.0, 2.0));
+            == Denote(Unit);
+        }
+    }
+    
+    // Look ma, no proof!
+    lemma IntersectUnitTest()
+        ensures Denote(Intersect(Unit, Translate(1.0, Unit))) == Denote(Empty)
+    {}
+    
+    lemma OpenDenoteOpen(e: Expr)
+        ensures Open(OpenDenote(e))
+    {
+        match e {
+            case Empty =>
+            case Unit => OpenIntervalOpen(0.0, 1.0);
+            case Translate(r, e) => TranslateSetOpen(r, OpenDenote(e));
+            case Home(r, e) => var S := OpenDenote(e);
+                TranslateSetOpen(-RelPos(r, S), S);
+            case Scale(r, e) => { ScaleSetOpen(r, OpenDenote(e)); }
+            case Intersect(e1, e2) => {}
+            case Union(e1, e2) => {}
+            case Difference(e1, e2) => { DifferenceOpen(OpenDenote(e1), OpenDenote(e2)); }
+        }
+    }
+    
+    predicate NoIsolatedPoints(S: iset<real>)
+    {
+        forall x, eps | x in S && eps > 0.0 :: !((Ball(x, eps) - iset{x}) !! S)
+    }
+    
+    lemma DenoteNoIsolatedPoints(e: Expr)
+        ensures NoIsolatedPoints(Denote(e))
+    {
+        forall x, eps | x in Denote(e) && eps > 0.0
+            ensures exists z :: z in Ball(x, eps) && z != x && z in Denote(e)
         {
-            assert OpenDenote(e1) * OpenDenote(e2) ==
-                OpenDenote(e1) - Closure(OpenDenote(e1) - Closure(OpenDenote(e2)))
-            by {
-                var S1 := OpenDenote(e1);
-                var S2 := OpenDenote(e2);
-                OpenDenoteOpen(e2);
-                
-                forall x | x in S1 && x in S2
-                    ensures x in S1 - Closure(S1 - Closure(S2))
-                {
-                    var eps :| Ball(x, eps) <= S2;
-                }
-                forall x | x in S1 && x !in Closure(S1 - Closure(S2))
-                    ensures x in S1 * S2
-                {}
+            assert !(OpenDenote(e) !! Ball(x, eps / 2.0));
+            var y :| y in OpenDenote(e) && y in Ball(x, eps / 2.0);
+            if x == y {
+                OpenDenoteOpen(e);
+                var eps' :| eps' > 0.0 && Ball(y, eps') <= OpenDenote(e);
+                var eps'' := min(eps, eps') / 2.0;
+                var z := x + eps'';
+                assert z in Ball(y, eps');
+                assert z in Denote(e);
+            } else {
+                assert y in Denote(e);
+            }
+    
+        }
+    }
+    
+    predicate HasNearbyPointInInterior(S: iset<real>, x: real, eps: real)
+    {
+        exists x', eps' | eps' > 0.0 :: Ball(x', eps') <= (Ball(x, eps) * S)
+    }
+    
+    predicate NoInfinitelyThinFeatures(S: iset<real>)
+    {
+        forall x, eps | x in S && eps > 0.0 ::
+            HasNearbyPointInInterior(S, x, eps)
+    }
+    
+    lemma DenoteNoInfinitelyThinFeatures(e: Expr)
+        ensures NoInfinitelyThinFeatures(Denote(e))
+    {
+        var S := Denote(e);
+        forall x, eps | x in S && eps > 0.0
+            ensures HasNearbyPointInInterior(S, x, eps)
+        {
+            assert x in Closure(OpenDenote(e));
+            var x' :| x' in Ball(x, eps) && x' in OpenDenote(e);
+            OpenDenoteOpen(e);
+            var eps' :| eps' > 0.0 && Ball(x', eps') <= OpenDenote(e);
+    
+            var eps'' := min(eps', eps - abs(x - x'));
+            assert Ball(x', eps'') <= OpenDenote(e);
+        }
+    }
+    
+    predicate AlternativeNoInfinitelyThinFeatures(S: iset<real>)
+    {
+        S <= Closure(Interior(S))
+    }
+    
+    lemma AlternativeNoInfinitelyThinFeaturesEquiv(S: iset<real>)
+        ensures AlternativeNoInfinitelyThinFeatures(S) <==> NoInfinitelyThinFeatures(S)
+    {
+        if AlternativeNoInfinitelyThinFeatures(S) {
+            forall x, eps | x in S && eps > 0.0
+                ensures HasNearbyPointInInterior(S, x, eps)
+            {
+                var x' :| x' in Ball(x, eps) && x' in Interior(S);
+                var eps' :| eps' > 0.0 && Ball(x', eps') <= S;
+                var eps'' := min(eps', eps - abs(x - x'));
+                assert Ball(x', eps'') <= Ball(x, eps);
             }
         }
-        Closure(OpenDenote(e1) - Closure(OpenDenote(e1) - Closure(OpenDenote(e2))));
-        Closure(OpenDenote(Difference(e1, Difference(e1, e2))));
-        Denote(Difference(e1, Difference(e1, e2)));
+    
+        if NoInfinitelyThinFeatures(S) {
+            forall x | x in S
+                ensures x in Closure(Interior(S))
+            {
+                forall eps | eps > 0.0
+                    ensures !(Ball(x, eps) !! Interior(S))
+                {
+                    assert HasNearbyPointInInterior(S, x, eps);
+                    var x', eps' :| eps' > 0.0 && Ball(x', eps') <= (Ball(x, eps) * S);
+                    assert x' in Ball(x', eps');
+                }
+            }
+        }
+    }
+    
+    function RelPos(r: real, S: iset<real>): real
+        requires Bounded(S)
+    {
+        if S == iset{} then
+            0.0  // dummy value
+        else
+            var (a, b) := BBox(S);
+            a + r * (b - a)
+    }
+    
+    predicate Equiv(e1: Expr, e2: Expr)
+    {
+        Denote(e1) == Denote(e2)
+    }
+    
+    lemma SelfUnion(e: Expr)
+        ensures Equiv(Union(e, e), e)
+    {}
+    
+    lemma SelfIntersect(e: Expr)
+        ensures Equiv(Intersect(e, e), e)
+    {}
+    
+    lemma SelfDifference(e: Expr)
+        ensures Equiv(Difference(e, e), Empty)
+    {}
+    
+    lemma UnionEmpty(e: Expr)
+        ensures Equiv(Union(e, Empty), e)
+    {}
+    
+    lemma IntersectEmpty(e: Expr)
+        ensures Equiv(Intersect(e, Empty), Empty)
+    {}
+    
+    
+    lemma DifferenceEmpty1(e: Expr)
+        ensures Equiv(Difference(e, Empty), e)
+    {
+        calc {
+            Denote(Difference(e, Empty));
+            Closure(OpenDenote(e) - Closure(iset{}));
+            { ClosureEmpty(); }
+            Closure(OpenDenote(e));
+            Denote(e);
+        }
+    }
+    
+    lemma DifferenceEmpty2(e: Expr)
+        ensures Equiv(Difference(Empty, e), Empty)
+    {}
+    
+    lemma UnionComm(e1: Expr, e2: Expr)
+        ensures Equiv(Union(e1, e2), Union(e2, e1))
+    {}
+    
+    lemma IntersectComm(e1: Expr, e2: Expr)
+        ensures Equiv(Intersect(e1, e2), Intersect(e2, e1))
+    {}
+    
+    lemma UnionAssoc(e1: Expr, e2: Expr, e3: Expr)
+        ensures Equiv(Union(e1, Union(e2, e3)), Union(Union(e1, e2), e3))
+    {
+        assert
+            OpenDenote(e1) + (OpenDenote(e2) + OpenDenote(e3)) ==
+            (OpenDenote(e1) + OpenDenote(e2)) + OpenDenote(e3);
+    }
+    
+    lemma IntersectAssoc(e1: Expr, e2: Expr, e3: Expr)
+        ensures Equiv(Intersect(e1, Intersect(e2, e3)), Intersect(Intersect(e1, e2), e3))
+    {
+        assert
+            OpenDenote(e1) * (OpenDenote(e2) * OpenDenote(e3)) ==
+            (OpenDenote(e1) * OpenDenote(e2)) * OpenDenote(e3);
+    }
+    
+    lemma IntersectDifference(e1: Expr, e2: Expr)
+        ensures Equiv(Intersect(e1, e2), Difference(e1, Difference(e1, e2)));
+    {
+        calc {
+            Denote(Intersect(e1, e2));
+            Closure(OpenDenote(Intersect(e1, e2)));
+            Closure(OpenDenote(e1) * OpenDenote(e2));
+            {
+                assert OpenDenote(e1) * OpenDenote(e2) ==
+                    OpenDenote(e1) - Closure(OpenDenote(e1) - Closure(OpenDenote(e2)))
+                by {
+                    var S1 := OpenDenote(e1);
+                    var S2 := OpenDenote(e2);
+                    OpenDenoteOpen(e2);
+                    
+                    forall x | x in S1 && x in S2
+                        ensures x in S1 - Closure(S1 - Closure(S2))
+                    {
+                        var eps :| Ball(x, eps) <= S2;
+                    }
+                    forall x | x in S1 && x !in Closure(S1 - Closure(S2))
+                        ensures x in S1 * S2
+                    {}
+                }
+            }
+            Closure(OpenDenote(e1) - Closure(OpenDenote(e1) - Closure(OpenDenote(e2))));
+            Closure(OpenDenote(Difference(e1, Difference(e1, e2))));
+            Denote(Difference(e1, Difference(e1, e2)));
+        }
     }
 }
